Tidy up Montgomery ladders
This simplifies the remaining Montgomery ladder implementations by
avoiding the special code for zero handling, since it is not actually
necessary given the behavior of the modular inverse in this case. In
addition, the proofs have been tidied up a bit, factoring out the
basic mathematics so that the loop invariant becomes simpler.

The update also fixes a README typo pointed out by Dan Bernstein
and removes a couple of stray comments arising from SLOTHY output
in the Lenngren-derived X25519 code.

arm/proofs/curve25519_x25519_byte_alt.ml
@@ -2761,23 +2761,17 @@ let curve25519_x25519_byte_alt_mc = define_assert_from_elf
   0xab0401ef;       (* arm_ADDS X15 X15 X4 *)
   0x9a050210;       (* arm_ADC X16 X16 X5 *)
   0xab0f01ff;       (* arm_CMN X15 X15 *)
-  0xb24101ef;       (* arm_ORR X15 X15 (rvalue (word 9223372036854775808)) *)
+  0x9240f9ef;       (* arm_AND X15 X15 (rvalue (word 9223372036854775807)) *)
   0x9a100208;       (* arm_ADC X8 X16 X16 *)
   0xd2800267;       (* arm_MOV X7 (rvalue (word 19)) *)
-  0x9b081ceb;       (* arm_MADD X11 X7 X8 X7 *)
+  0x9b087ceb;       (* arm_MUL X11 X7 X8 *)
   0xab0b018c;       (* arm_ADDS X12 X12 X11 *)
   0xba0901ad;       (* arm_ADCS X13 X13 X9 *)
   0xba0301ce;       (* arm_ADCS X14 X14 X3 *)
-  0xba1f01ef;       (* arm_ADCS X15 X15 XZR *)
-  0x9a9f30e7;       (* arm_CSEL X7 X7 XZR Condition_CC *)
-  0xeb07018c;       (* arm_SUBS X12 X12 X7 *)
-  0xfa1f01ad;       (* arm_SBCS X13 X13 XZR *)
-  0xfa1f01ce;       (* arm_SBCS X14 X14 XZR *)
-  0xda1f01ef;       (* arm_SBC X15 X15 XZR *)
-  0x9240f9ef;       (* arm_AND X15 X15 (rvalue (word 9223372036854775807)) *)
+  0x9a1f01ef;       (* arm_ADC X15 X15 XZR *)
   0xa90a37ec;       (* arm_STP X12 X13 SP (Immediate_Offset (iword (&160))) *)
   0xa90b3fee;       (* arm_STP X14 X15 SP (Immediate_Offset (iword (&176))) *)
-  0x910383e0;       (* arm_ADD X0 SP (rvalue (word 224)) *)
+  0x910283e0;       (* arm_ADD X0 SP (rvalue (word 160)) *)
   0x910283e1;       (* arm_ADD X1 SP (rvalue (word 160)) *)
   0xaa0003f4;       (* arm_MOV X20 X0 *)
   0x9280024a;       (* arm_MOVN X10 (word 18) 0 *)
@@ -3805,28 +3799,14 @@ let curve25519_x25519_byte_alt_mc = define_assert_from_elf
   0xaa1403e4;       (* arm_MOV X4 X20 *)
   0xa9000480;       (* arm_STP X0 X1 X4 (Immediate_Offset (iword (&0))) *)
   0xa9011482;       (* arm_STP X2 X5 X4 (Immediate_Offset (iword (&16))) *)
-  0xa94a07e0;       (* arm_LDP X0 X1 SP (Immediate_Offset (iword (&160))) *)
-  0xa94b0fe2;       (* arm_LDP X2 X3 SP (Immediate_Offset (iword (&176))) *)
-  0xaa010000;       (* arm_ORR X0 X0 X1 *)
-  0xaa030042;       (* arm_ORR X2 X2 X3 *)
-  0xaa020004;       (* arm_ORR X4 X0 X2 *)
-  0xeb1f009f;       (* arm_CMP X4 XZR *)
-  0xa95207e0;       (* arm_LDP X0 X1 SP (Immediate_Offset (iword (&288))) *)
-  0x9a9f1000;       (* arm_CSEL X0 X0 XZR Condition_NE *)
-  0x9a9f1021;       (* arm_CSEL X1 X1 XZR Condition_NE *)
-  0xa9530fe2;       (* arm_LDP X2 X3 SP (Immediate_Offset (iword (&304))) *)
-  0xa91207e0;       (* arm_STP X0 X1 SP (Immediate_Offset (iword (&288))) *)
-  0x9a9f1042;       (* arm_CSEL X2 X2 XZR Condition_NE *)
-  0x9a9f1063;       (* arm_CSEL X3 X3 XZR Condition_NE *)
-  0xa9130fe2;       (* arm_STP X2 X3 SP (Immediate_Offset (iword (&304))) *)
   0xa95213e3;       (* arm_LDP X3 X4 SP (Immediate_Offset (iword (&288))) *)
-  0xa94e23e7;       (* arm_LDP X7 X8 SP (Immediate_Offset (iword (&224))) *)
+  0xa94a23e7;       (* arm_LDP X7 X8 SP (Immediate_Offset (iword (&160))) *)
   0x9b077c6c;       (* arm_MUL X12 X3 X7 *)
   0x9bc77c6d;       (* arm_UMULH X13 X3 X7 *)
   0x9b087c6b;       (* arm_MUL X11 X3 X8 *)
   0x9bc87c6e;       (* arm_UMULH X14 X3 X8 *)
   0xab0b01ad;       (* arm_ADDS X13 X13 X11 *)
-  0xa94f2be9;       (* arm_LDP X9 X10 SP (Immediate_Offset (iword (&240))) *)
+  0xa94b2be9;       (* arm_LDP X9 X10 SP (Immediate_Offset (iword (&176))) *)
   0x9b097c6b;       (* arm_MUL X11 X3 X9 *)
   0x9bc97c6f;       (* arm_UMULH X15 X3 X9 *)
   0xba0b01ce;       (* arm_ADCS X14 X14 X11 *)
@@ -3991,20 +3971,6 @@ let curve25519_x25519_byte_alt_mc = define_assert_from_elf
 let CURVE25519_X25519_BYTE_ALT_EXEC = ARM_MK_EXEC_RULE curve25519_x25519_byte_alt_mc;;
 
 (* ------------------------------------------------------------------------- *)
-(* Abbreviations used to state the specification.                            *)
-(* ------------------------------------------------------------------------- *)
-
-let p_25519 = define `p_25519 = 57896044618658097711785492504343953926634992332820282019728792003956564819949`;;
-
-let curve25519x = define
- `curve25519x (f:A ring) = (f,ring_of_num f A_25519,ring_of_num f 1)`;;
-
-let curve25519x_halfcanonically_represents = new_definition
- `curve25519x_halfcanonically_represents (f:A ring) P (X,Z) <=>
-        X < 2 * p_25519 /\ Z < 2 * p_25519 /\
-        montgomery_xz f P (ring_of_num f X,ring_of_num f Z)`;;
-
-(* ------------------------------------------------------------------------- *)
 (* Common lemmas and tactics for the component proofs.                       *)
 (* ------------------------------------------------------------------------- *)
 
@@ -4048,7 +4014,7 @@ let LOCAL_MUL_P25519_TAC =
       !n. read(memory :> bytes(word_add (read p2 t) (word n2),8 * 4)) t = n
       ==>
       aligned 16 (read SP t) /\
-      nonoverlapping (word pc,0x3de4) (word_add (read p3 t) (word n3),8 * 4)
+      nonoverlapping (word pc,0x3d94) (word_add (read p3 t) (word n3),8 * 4)
       ==> ensures arm
            (\s. aligned_bytes_loaded s (word pc) curve25519_x25519_byte_alt_mc /\
                 read PC s = pcin /\
@@ -4211,7 +4177,7 @@ let LOCAL_MUL_4_TAC =
       !n. read(memory :> bytes(word_add (read p2 t) (word n2),8 * 4)) t = n
       ==>
       aligned 16 (read SP t) /\
-      nonoverlapping (word pc,0x3de4) (word_add (read p3 t) (word n3),8 * 4)
+      nonoverlapping (word pc,0x3d94) (word_add (read p3 t) (word n3),8 * 4)
       ==> ensures arm
            (\s. aligned_bytes_loaded s (word pc) curve25519_x25519_byte_alt_mc /\
                 read PC s = pcin /\
@@ -4364,7 +4330,7 @@ let LOCAL_SQR_4_TAC =
       read(memory :> bytes(word_add (read p1 t) (word n1),8 * 4)) t = n
       ==>
       aligned 16 (read SP t) /\
-      nonoverlapping (word pc,0x3de4) (word_add (read p3 t) (word n3),8 * 4)
+      nonoverlapping (word pc,0x3d94) (word_add (read p3 t) (word n3),8 * 4)
       ==> ensures arm
            (\s. aligned_bytes_loaded s (word pc) curve25519_x25519_byte_alt_mc /\
                 read PC s = pcin /\
@@ -4519,7 +4485,7 @@ let LOCAL_ADD_TWICE4_TAC =
       !n. read(memory :> bytes(word_add (read p2 t) (word n2),8 * 4)) t = n
       ==>
       aligned 16 (read SP t) /\
-      nonoverlapping (word pc,0x3de4) (word_add (read p3 t) (word n3),8 * 4)
+      nonoverlapping (word pc,0x3d94) (word_add (read p3 t) (word n3),8 * 4)
       ==> ensures arm
            (\s. aligned_bytes_loaded s (word pc) curve25519_x25519_byte_alt_mc /\
                 read PC s = pcin /\
@@ -4592,7 +4558,7 @@ let LOCAL_SUB_TWICE4_TAC =
       !n. read(memory :> bytes(word_add (read p2 t) (word n2),8 * 4)) t = n
       ==>
       aligned 16 (read SP t) /\
-      nonoverlapping (word pc,0x3de4) (word_add (read p3 t) (word n3),8 * 4)
+      nonoverlapping (word pc,0x3d94) (word_add (read p3 t) (word n3),8 * 4)
       ==> ensures arm
            (\s. aligned_bytes_loaded s (word pc) curve25519_x25519_byte_alt_mc /\
                 read PC s = pcin /\
@@ -4671,7 +4637,7 @@ let LOCAL_CMADD_4_TAC =
      !n. read(memory :> bytes(word_add (read p2 t) (word n2),8 * 4)) t = n
      ==>
       aligned 16 (read SP t) /\
-      nonoverlapping (word pc,0x3de4) (word_add (read p3 t) (word n3),8 * 4)
+      nonoverlapping (word pc,0x3d94) (word_add (read p3 t) (word n3),8 * 4)
       ==> ensures arm
            (\s. aligned_bytes_loaded s (word pc) curve25519_x25519_byte_alt_mc /\
                 read PC s = pcin /\
@@ -4815,7 +4781,7 @@ let LOCAL_MUX_4_TAC =
      !n. read(memory :> bytes(word_add (read p2 t) (word n2),8 * 4)) t = n
      ==>
       aligned 16 (read SP t) /\
-      nonoverlapping (word pc,0x3de4) (word_add (read p3 t) (word n3),8 * 4) /\
+      nonoverlapping (word pc,0x3d94) (word_add (read p3 t) (word n3),8 * 4) /\
       nonoverlapping (stackpointer:int64,320) (res,32)
       ==> ensures arm
            (\s. aligned_bytes_loaded s (word pc) curve25519_x25519_byte_alt_mc /\
@@ -4846,104 +4812,279 @@ let LOCAL_MUX_4_TAC =
 
 let LOCAL_MODINV_TAC =
   ARM_SUBROUTINE_SIM_TAC
-   (curve25519_x25519_byte_alt_mc,CURVE25519_X25519_BYTE_ALT_EXEC,0x2b08,
+   (curve25519_x25519_byte_alt_mc,CURVE25519_X25519_BYTE_ALT_EXEC,0x2af0,
     (GEN_REWRITE_CONV RAND_CONV [bignum_inv_p25519_mc] THENC TRIM_LIST_CONV)
     `TRIM_LIST (12,16) bignum_inv_p25519_mc`,
     CORE_INV_P25519_CORRECT)
    [`read X0 s`; `read X1 s`;
     `read (memory :> bytes(read X1 s,8 * 4)) s`;
-    `pc + 0x2b08`; `stackpointer:int64`];;
+    `pc + 0x2af0`; `stackpointer:int64`];;
+
+(* ------------------------------------------------------------------------- *)
+(* The swapping-based Montgomery ladder more abstractly.                     *)
+(* ------------------------------------------------------------------------- *)
+
+(*** This version has the i = 0 split to handle the short-cut of the
+ *** 255th bit, where the values are not exactly the same as the usual
+ *** ladder, just projectively equivalent to them.
+ ***)
+
+let flipladder = define
+ `flipladder x n 0 = ((&1,&0),(&x rem &p_25519,&1)) /\
+  flipladder x n (i + 1) =
+        let (x2,z2),(x3,z3) = flipladder x n i in
+        montgomery_xzdouble curve25519
+          (if ODD(n DIV 2 EXP (255 - (i + 1))) <=> ODD(n DIV 2 EXP (255 - i))
+           then (x2,z2) else (x3,z3)),
+        (if i = 0 then (&x rem &p_25519,&1)
+         else montgomery_xzdiffadd curve25519 (&x,&1) (x2,z2) (x3,z3))`;;
+
+let ladder_x2 = define
+  `ladder_x2 x n i = FST(FST(flipladder x n (255 - i)))`;;
+
+let ladder_z2 = define
+  `ladder_z2 x n i = SND(FST(flipladder x n (255 - i)))`;;
+
+let ladder_x3 = define
+  `ladder_x3 x n i = FST(SND(flipladder x n (255 - i)))`;;
+
+let ladder_z3 = define
+  `ladder_z3 x n i = SND(SND(flipladder x n (255 - i)))`;;
+
+let deproject = define
+ `deproject (x,z) =
+   (x * (if p_25519 divides z then 0 else inverse_mod p_25519 z))
+   MOD p_25519`;;
+
+let curve25519x_represents = define
+ `curve25519x_represents (f:A ring) P n (X,Z) <=>
+        P IN group_carrier(montgomery_group (curve25519x f)) /\
+        montgomery_xz f (group_pow (montgomery_group (curve25519x f)) P n)
+                        (ring_of_int f X,ring_of_int f Z)`;;
+
+let CURVE25519X_REPRESENTS_DOUBLE = prove
+ (`!(f:A ring) P n Q.
+        field f /\ ring_char f = p_25519 /\
+        curve25519x_represents f P n Q
+        ==> curve25519x_represents f P (2 * n)
+                (montgomery_xzdouble curve25519 Q)`,
+  REWRITE_TAC[FORALL_PAIR_THM; curve25519x_represents] THEN
+  MAP_EVERY X_GEN_TAC
+   [`f:A ring`; `P:(A#A)option`; `n:num`; `X:int`; `Z:int`] THEN
+  STRIP_TAC THEN GEN_REWRITE_TAC RAND_CONV [GSYM PAIR] THEN
+  PURE_REWRITE_TAC[curve25519x_represents] THEN ASM_REWRITE_TAC[] THEN
+  MP_TAC(ISPECL
+   [`f:A ring`; `ring_of_num (f:A ring) A_25519`; `ring_of_num (f:A ring) 1`;
+    `P:(A#A)option`; `n:num`; `ring_of_int f X:A,ring_of_int f Z`]
+   MONTGOMERY_XZDOUBLE_GROUP) THEN
+  ASM_SIMP_TAC[GSYM curve25519x; MONTGOMERY_NONSINGULAR_CURVE25519X] THEN
+  REWRITE_TAC[RING_OF_NUM; p_25519; ARITH_EQ] THEN
+  MATCH_MP_TAC EQ_IMP THEN AP_TERM_TAC THEN
+  REWRITE_TAC[montgomery_xzdouble; curve25519x; curve25519] THEN
+  REWRITE_TAC[INTEGER_MOD_RING_CLAUSES; PAIR_EQ] THEN
+  CONV_TAC INT_REM_DOWN_CONV THEN
+  FIRST_X_ASSUM(SUBST1_TAC o SYM) THEN
+  REWRITE_TAC[RING_OF_INT_REM] THEN
+  REWRITE_TAC[GSYM RING_OF_INT_CLAUSES] THEN
+  REWRITE_TAC[RING_OF_INT_OF_NUM]);;
+
+let CURVE25519X_REPRESENTS_DIFFADD_LEFT = prove
+ (`!(f:A ring) P n X Qm Qn.
+        field f /\ ring_char f = p_25519 /\ ~(&p_25519 divides X) /\
+        curve25519x_represents f P 1 (X,&1) /\
+        curve25519x_represents f P (n + 1) Qm /\
+        curve25519x_represents f P n Qn
+        ==> curve25519x_represents f P (2 * n + 1)
+                (montgomery_xzdiffadd curve25519 (X,&1) Qm Qn)`,
+  REWRITE_TAC[FORALL_PAIR_THM; curve25519x_represents] THEN
+  MAP_EVERY X_GEN_TAC
+   [`f:A ring`; `P:(A#A)option`; `n:num`; `X:int`;
+    `Xm:int`; `Zm:int`; `Xn:int`; `Zn:int`] THEN
+  STRIP_TAC THEN GEN_REWRITE_TAC RAND_CONV [GSYM PAIR] THEN
+  PURE_REWRITE_TAC[curve25519x_represents] THEN ASM_REWRITE_TAC[] THEN
+  MP_TAC(ISPECL
+   [`f:A ring`; `ring_of_num (f:A ring) A_25519`; `ring_of_num (f:A ring) 1`;
+    `P:(A#A)option`; `n:num`;
+    `ring_of_int f X:A,ring_of_int f (&1)`;
+    `ring_of_int f Xm:A,ring_of_int f Zm`;
+    `ring_of_int f Xn:A,ring_of_int f Zn`]
+   MONTGOMERY_XZDIFFADD_GROUP) THEN
+  ASM_SIMP_TAC[GSYM curve25519x; MONTGOMERY_NONSINGULAR_CURVE25519X] THEN
+  ASM_REWRITE_TAC[RING_OF_NUM; p_25519; ARITH_EQ] THEN ANTS_TAC THENL
+   [ASM_REWRITE_TAC[RING_OF_INT_EQ_0] THEN
+    REWRITE_TAC[GSYM num_divides; DIVIDES_MOD; p_25519] THEN
+    CONV_TAC NUM_REDUCE_CONV THEN ASM_MESON_TAC[GROUP_POW_1];
+    MATCH_MP_TAC EQ_IMP THEN AP_TERM_TAC] THEN
+  REWRITE_TAC[montgomery_xzdiffadd; curve25519x; curve25519] THEN
+  REWRITE_TAC[INTEGER_MOD_RING_CLAUSES; PAIR_EQ] THEN
+  CONV_TAC INT_REM_DOWN_CONV THEN
+  FIRST_X_ASSUM(SUBST1_TAC o SYM) THEN
+  REWRITE_TAC[RING_OF_INT_REM] THEN
+  REWRITE_TAC[GSYM RING_OF_INT_CLAUSES] THEN
+  REWRITE_TAC[RING_OF_INT_OF_NUM]);;
+
+let CURVE25519X_REPRESENTS_DIFFADD_RIGHT = prove
+ (`!(f:A ring) P n X Qm Qn.
+        field f /\ ring_char f = p_25519 /\ ~(&p_25519 divides X) /\
+        curve25519x_represents f P 1 (X,&1) /\
+        curve25519x_represents f P n Qm /\
+        curve25519x_represents f P (n + 1) Qn
+        ==> curve25519x_represents f P (2 * n + 1)
+                (montgomery_xzdiffadd curve25519 (X,&1) Qm Qn)`,
+  REWRITE_TAC[FORALL_PAIR_THM] THEN REPEAT GEN_TAC THEN
+  ONCE_REWRITE_TAC[TAUT
+   `p /\ q /\ r /\ s /\ t /\ u <=> p /\ q /\ r /\ s /\ u /\ t`] THEN
+  DISCH_TAC THEN
+  FIRST_ASSUM(MP_TAC o MATCH_MP CURVE25519X_REPRESENTS_DIFFADD_LEFT) THEN
+  MATCH_MP_TAC EQ_IMP THEN AP_TERM_TAC THEN
+  REWRITE_TAC[montgomery_xzdiffadd; curve25519] THEN
+  REWRITE_TAC[PAIR_EQ; INTEGER_MOD_RING_CLAUSES] THEN CONJ_TAC THEN
+  CONV_TAC INT_REM_DOWN_CONV THEN AP_THM_TAC THEN AP_TERM_TAC THEN
+  INT_ARITH_TAC);;
+
+let FLIPLADDER_MAIN = prove
+ (`!(f:A ring) P x n i.
+        field f /\ ring_char f = p_25519 /\ ~(p_25519 divides x) /\
+        curve25519x_represents f P 1 (&x,&1) /\
+        n < 2 EXP 255 /\ n DIV 2 EXP 254 = 1 /\ i <= 255
+        ==> curve25519x_represents f P (n DIV 2 EXP (255 - i))
+                ((if ODD(n DIV 2 EXP (255 - i)) then SND else FST)
+                 (flipladder x n i)) /\
+            curve25519x_represents f P (n DIV 2 EXP (255 - i) + 1)
+                ((if ODD(n DIV 2 EXP (255 - i)) then FST else SND)
+                 (flipladder x n i))`,
+  REWRITE_TAC[num_divides] THEN REPLICATE_TAC 4 GEN_TAC THEN
+  REWRITE_TAC[IMP_CONJ; RIGHT_FORALL_IMP_THM] THEN REPEAT DISCH_TAC THEN
+  INDUCT_TAC THENL
+   [DISCH_THEN(K ALL_TAC) THEN POP_ASSUM(K ALL_TAC) THEN
+    REWRITE_TAC[flipladder] THEN
+    ASM_SIMP_TAC[SUB_0; DIV_LT; ARITH_ODD; ADD_CLAUSES] THEN
+    FIRST_X_ASSUM(MP_TAC o GEN_REWRITE_RULE I [curve25519x_represents]) THEN
+    SIMP_TAC[curve25519x_represents; group_pow] THEN DISCH_TAC THEN
+    FIRST_ASSUM(SUBST1_TAC o SYM) THEN REWRITE_TAC[RING_OF_INT_REM] THEN
+    STRIP_TAC THEN ASM_SIMP_TAC[CURVE25519X_GROUP; GSYM curve25519x_group] THEN
+    REWRITE_TAC[montgomery_xz; RING_OF_INT_1; RING_OF_INT_0] THEN
+    REWRITE_TAC[RING_0; RING_1] THEN ASM_MESON_TAC[field];
+    DISCH_TAC THEN FIRST_X_ASSUM(MP_TAC o check (is_imp o concl)) THEN
+    ANTS_TAC THENL [ASM_ARITH_TAC; ALL_TAC]] THEN
+  REWRITE_TAC[flipladder; ADD1] THEN
+  ASM_SIMP_TAC[ARITH_RULE
+     `SUC i <= 255 ==> 255 - i = SUC(255 - (i + 1))`] THEN
+  REWRITE_TAC[ONCE_REWRITE_RULE[MULT_SYM] (CONJUNCT2 EXP)] THEN
+  ASM_CASES_TAC `i = 0` THEN ASM_REWRITE_TAC[] THENL
+   [ASM_REWRITE_TAC[ADD_CLAUSES; ARITH_RULE `255 - 1 = 254`] THEN
+    ASM_SIMP_TAC[DIV_LT; ARITH_RULE `2 EXP 254 * 2 = 2 EXP 255`] THEN
+    LET_TAC THEN CONV_TAC(ONCE_DEPTH_CONV let_CONV) THEN
+    CONV_TAC NUM_REDUCE_CONV THEN REWRITE_TAC[] THEN
+    SUBST1_TAC(ARITH_RULE `2 = 2 * 1`) THEN
+    ASM_SIMP_TAC[CURVE25519X_REPRESENTS_DOUBLE] THEN
+    DISCH_THEN(K ALL_TAC) THEN
+    FIRST_X_ASSUM(MP_TAC o GEN_REWRITE_RULE I [curve25519x_represents]) THEN
+    SIMP_TAC[curve25519x_represents] THEN ASM_MESON_TAC[RING_OF_INT_REM];
+    ALL_TAC] THEN
+  REWRITE_TAC[GSYM DIV_DIV] THEN
+  ABBREV_TAC `m = n DIV 2 EXP (255 - (i + 1)) DIV 2` THEN
+  MP_TAC(SPECL [`n DIV 2 EXP (255 - (i + 1))`; `2`]
+   (CONJUNCT1 DIVISION_SIMP)) THEN
+  ASM_REWRITE_TAC[MOD_2_CASES; GSYM NOT_ODD; COND_SWAP] THEN
+  MAP_EVERY ABBREV_TAC
+   [`b <=> ODD m`; `c <=> ODD(n DIV 2 EXP (255 - (i + 1)))`] THEN
+  DISCH_THEN(SUBST1_TAC o SYM) THEN
+  MAP_EVERY ASM_CASES_TAC [`b:bool`; `c:bool`] THEN
+  ASM_REWRITE_TAC[] THEN LET_TAC THEN ASM_REWRITE_TAC[] THEN
+  CONV_TAC(ONCE_DEPTH_CONV let_CONV) THEN ASM_REWRITE_TAC[] THEN
+  REWRITE_TAC[ADD_CLAUSES; ARITH_RULE `m * 2 = 2 * m`;
+              ARITH_RULE `(2 * m + 1) + 1 = 2 * (m + 1)`] THEN
+  ASM_MESON_TAC[CURVE25519X_REPRESENTS_DOUBLE;
+        CURVE25519X_REPRESENTS_DIFFADD_LEFT;
+        CURVE25519X_REPRESENTS_DIFFADD_RIGHT]);;
+
+let FLIPLADDER_DEGENERATE = prove
+ (`!x n i xm zm xn zn.
+        p_25519 divides x /\ flipladder x n i = (xm,zm),(xn,zn)
+        ==> zm = &0 /\ xn = &0`,
+  GEN_TAC THEN GEN_TAC THEN REWRITE_TAC[IMP_CONJ; RIGHT_FORALL_IMP_THM] THEN
+  REWRITE_TAC[num_divides; GSYM INT_REM_EQ_0] THEN DISCH_TAC THEN
+  INDUCT_TAC THEN ASM_SIMP_TAC[flipladder; PAIR_EQ] THENL
+   [MESON_TAC[]; REWRITE_TAC[flipladder; ADD1]] THEN
+  REPEAT GEN_TAC THEN LET_TAC THEN
+  SUBGOAL_THEN `z2:int = &0 /\ x3:int = &0` MP_TAC THENL
+   [ASM_MESON_TAC[]; REPLICATE_TAC 2 (POP_ASSUM(K ALL_TAC))] THEN
+  STRIP_TAC THEN REPEAT COND_CASES_TAC THEN
+  ASM_REWRITE_TAC[montgomery_xzdouble; curve25519; montgomery_xzdouble;
+                  PAIR_EQ; montgomery_xzdiffadd; INTEGER_MOD_RING_CLAUSES] THEN
+  CONV_TAC INT_REM_DOWN_CONV THEN
+  DISCH_THEN(fun th -> REWRITE_TAC[GSYM th]) THEN
+  REWRITE_TAC[INT_MUL_LZERO; INT_MUL_RZERO; INT_SUB_REFL; INT_POW_ZERO;
+              ARITH_EQ; INT_REM_ZERO]);;
+
+let DEPROJECT_LADDER_EVEN = prove
+ (`!x n x2 z2.
+        n < 2 EXP 255 /\ n DIV 2 EXP 254 = 1 /\ EVEN n /\
+        (&x2 == ladder_x2 x n 0) (mod &p_25519) /\
+        (&z2 == ladder_z2 x n 0) (mod &p_25519)
+        ==> purex25519(n,x) = deproject(x2,z2)`,
+  REWRITE_TAC[ladder_x2; ladder_z2; SUB_0] THEN REPEAT STRIP_TAC THEN
+  MATCH_MP_TAC PUREX25519_UNIQUE_IMP THEN CONJ_TAC THENL
+   [REWRITE_TAC[deproject; p_25519] THEN ARITH_TAC; ALL_TAC] THEN
+  MAP_EVERY X_GEN_TAC [`f:(int#int)ring`; `Q:((int#int)#(int#int))option`] THEN
+  STRIP_TAC THEN ASM_CASES_TAC `p_25519 divides x` THENL
+   [MP_TAC(ISPECL [`x:num`; `n:num`; `255`] FLIPLADDER_DEGENERATE) THEN
+    DISCH_THEN(MP_TAC o SPECL
+     [`ladder_x2 x n 0`; `ladder_z2 x n 0`;
+      `ladder_x3 x n 0`; `ladder_z3 x n 0`]) THEN
+    ASM_REWRITE_TAC[ladder_x2; ladder_z2; ladder_x3; ladder_z3] THEN
+    ASM_REWRITE_TAC[SUB_0] THEN DISCH_THEN(CONJUNCTS_THEN SUBST_ALL_TAC) THEN
+    ASM_REWRITE_TAC[deproject; num_divides; GSYM INT_CONG_0_DIVIDES] THEN
+    REWRITE_TAC[MULT_CLAUSES; MOD_0; RING_OF_NUM_0] THEN
+    REWRITE_TAC[curve25519x_group; curve25519x] THEN
+    MATCH_MP_TAC MONTGOMERY_XMAP_EQ_0_POW THEN
+    ASM_REWRITE_TAC[GSYM curve25519x_group; GSYM curve25519x; RING_OF_NUM] THEN
+    ASM_SIMP_TAC[MONTGOMERY_NONSINGULAR_CURVE25519X; RING_OF_NUM_EQ_0] THEN
+    REWRITE_TAC[p_25519; ARITH_EQ];
+    ALL_TAC] THEN
+  MP_TAC(ISPECL [`f:(int#int)ring`; `Q:((int#int)#(int#int))option`;
+                 `x:num`; `n:num`; `255`]
+         FLIPLADDER_MAIN) THEN
+  ASM_REWRITE_TAC[SUB_REFL; EXP; DIV_1; LE_REFL] THEN ANTS_TAC THENL
+   [ASM_SIMP_TAC[curve25519x_represents; GROUP_POW_1;
+      GSYM curve25519x_group; RING_OF_INT_OF_NUM; RING_OF_NUM_1] THEN
+    ASM_SIMP_TAC[MONTGOMERY_XZ_XMAP; RING_OF_NUM_EQ_0; RING_OF_NUM];
+    DISCH_THEN(MP_TAC o CONJUNCT1) THEN ASM_REWRITE_TAC[GSYM NOT_EVEN]] THEN
+  GEN_REWRITE_TAC (LAND_CONV o RAND_CONV) [GSYM PAIR] THEN
+  REWRITE_TAC[curve25519x_represents] THEN
+  ONCE_REWRITE_TAC[GSYM RING_OF_INT_REM] THEN
+  ASM_REWRITE_TAC[GSYM curve25519x_group] THEN
+  REPEAT(FIRST_X_ASSUM(SUBST1_TAC o SYM o
+        GEN_REWRITE_RULE I [GSYM INT_REM_EQ])) THEN
+  SUBST1_TAC(SYM(ASSUME `ring_char(f:(int#int)ring) = p_25519`)) THEN
+  REWRITE_TAC[RING_OF_INT_REM; RING_OF_INT_OF_NUM] THEN
+  SPEC_TAC(`group_pow (curve25519x_group(f:(int#int)ring)) Q n`,
+           `P:((int#int)#(int#int))option`) THEN
+  MATCH_MP_TAC option_INDUCT THEN
+  GEN_REWRITE_TAC RAND_CONV [FORALL_PAIR_THM] THEN
+  ASM_SIMP_TAC[montgomery_xmap; montgomery_xz; deproject;
+               RING_OF_NUM_EQ_0; MULT_CLAUSES; MOD_0; RING_OF_NUM_0] THEN
+  X_GEN_TAC `y:int#int` THEN STRIP_TAC THEN
+  FIRST_X_ASSUM(SUBST1_TAC o SYM) THEN
+  SUBST1_TAC(SYM(ASSUME `ring_char(f:(int#int)ring) = p_25519`)) THEN
+  REWRITE_TAC[RING_OF_NUM_MOD; RING_OF_NUM_MUL; ring_div] THEN
+  AP_TERM_TAC THEN MATCH_MP_TAC RING_LINV_UNIQUE THEN
+  REWRITE_TAC[RING_OF_NUM; GSYM RING_OF_NUM_1] THEN
+  ASM_REWRITE_TAC[GSYM RING_OF_NUM_MUL; RING_OF_NUM_EQ] THEN
+  REWRITE_TAC[INVERSE_MOD_LMUL_EQ] THEN
+  ASM_SIMP_TAC[PRIME_COPRIME_EQ; PRIME_P25519]);;
 
 (* ------------------------------------------------------------------------- *)
 (* Overall point operation proof.                                            *)
 (* ------------------------------------------------------------------------- *)
 
-let nintlemma = prove
- (`&(num_of_int(x rem &p_25519)) = x rem &p_25519`,
-  MATCH_MP_TAC INT_OF_NUM_OF_INT THEN MATCH_MP_TAC INT_REM_POS THEN
-  REWRITE_TAC[INT_OF_NUM_EQ; p_25519] THEN CONV_TAC NUM_REDUCE_CONV);;
-
-let lemma = prove
- (`X = num_of_int(x rem &p_25519) ==> X < p_25519 /\ &X = x rem &p_25519`,
-  DISCH_THEN SUBST1_TAC THEN
-  REWRITE_TAC[GSYM INT_OF_NUM_LT; nintlemma; INT_LT_REM_EQ] THEN
-  REWRITE_TAC[INT_OF_NUM_LT; p_25519] THEN CONV_TAC NUM_REDUCE_CONV);;
-
-let lemma_double = prove
- (`P IN group_carrier (curve25519x_group(f:(int#int) ring)) /\
-   montgomery_xz f (group_pow (curve25519x_group f) P n) (x,y)
-   ==> field f /\ ring_char f = p_25519
-       ==> montgomery_xz f
-            (group_pow (curve25519x_group f) P (2 * n))
-               (montgomery_xzdouble (curve25519x f) (x,y))`,
-  REWRITE_TAC[curve25519x; curve25519x_group] THEN REPEAT STRIP_TAC THEN
-  MATCH_MP_TAC MONTGOMERY_XZDOUBLE_GROUP THEN ASM_REWRITE_TAC[] THEN
-  ASM_SIMP_TAC[GSYM curve25519x; MONTGOMERY_NONSINGULAR_CURVE25519X] THEN
-  REWRITE_TAC[A_25519; p_25519; RING_OF_NUM] THEN
-  CONV_TAC NUM_REDUCE_CONV);;
-
-let lemma_double_base = prove
- (`P IN group_carrier (curve25519x_group(f:(int#int) ring)) /\
-   montgomery_xz f P (x,y)
-   ==> field f /\ ring_char f = p_25519
-       ==> montgomery_xz f
-            (group_pow (curve25519x_group f) P 2)
-               (montgomery_xzdouble (curve25519x f) (x,y))`,
-  SUBST1_TAC(ARITH_RULE `2 = 2 * 1`) THEN
-  REWRITE_TAC[curve25519x; curve25519x_group] THEN REPEAT STRIP_TAC THEN
-  MATCH_MP_TAC MONTGOMERY_XZDOUBLE_GROUP THEN ASM_REWRITE_TAC[] THEN
-  ASM_SIMP_TAC[GROUP_POW_1] THEN
-  ASM_SIMP_TAC[GSYM curve25519x; MONTGOMERY_NONSINGULAR_CURVE25519X] THEN
-  REWRITE_TAC[A_25519; p_25519; RING_OF_NUM] THEN
-  CONV_TAC NUM_REDUCE_CONV);;
-
-let lemma_diffadd1 = prove
- (`field f /\ ring_char f = p_25519 /\
-   ~(x:(int#int) = ring_0 f) /\
-   P IN group_carrier (curve25519x_group f) /\
-   montgomery_xz f P (x,ring_of_num f 1) /\
-   montgomery_xz f
-     (group_pow (curve25519x_group f) P (n + 1)) (xn,zn) /\
-   montgomery_xz f
-     (group_pow (curve25519x_group f) P n) (xm,zm)
-   ==> montgomery_xz f
-            (group_pow (curve25519x_group f) P (2 * n + 1))
-            (montgomery_xzdiffadd (curve25519x f) (x,ring_of_num f 1)
-                  (xn,zn) (xm,zm))`,
-  REWRITE_TAC[curve25519x; curve25519x_group] THEN REPEAT STRIP_TAC THEN
-  MATCH_MP_TAC MONTGOMERY_XZDIFFADD_GROUP THEN ASM_REWRITE_TAC[] THEN
-  ASM_SIMP_TAC[GSYM curve25519x; MONTGOMERY_NONSINGULAR_CURVE25519X] THEN
-  REWRITE_TAC[A_25519; p_25519; RING_OF_NUM] THEN
-  ASM_SIMP_TAC[RING_OF_NUM_1; FIELD_NONTRIVIAL] THEN
-  CONV_TAC NUM_REDUCE_CONV);;
-
-let lemma_diffadd2 = prove
- (`field f /\ ring_char f = p_25519 /\
-   ~(x:(int#int) = ring_0 f) /\
-   P IN group_carrier (curve25519x_group f) /\
-   montgomery_xz f P (x,ring_of_num f 1) /\
-   montgomery_xz f
-     (group_pow (curve25519x_group f) P (n + 1)) (xm,zm) /\
-   montgomery_xz f
-     (group_pow (curve25519x_group f) P n) (xn,zn)
-   ==> montgomery_xz f
-            (group_pow (curve25519x_group f) P (2 * n + 1))
-            (montgomery_xzdiffadd (curve25519x f) (x,ring_of_num f 1)
-                  (xn,zn) (xm,zm))`,
-  DISCH_TAC THEN
-  FIRST_ASSUM(MP_TAC o MATCH_MP lemma_diffadd1) THEN
-  MATCH_MP_TAC EQ_IMP THEN AP_TERM_TAC THEN
-  POP_ASSUM STRIP_ASSUME_TAC THEN
-  REPEAT(FIRST_X_ASSUM(MP_TAC o MATCH_MP MONTGOMERY_XZ_IN_CARRIER)) THEN
-  ASM_SIMP_TAC[montgomery_xzdiffadd; curve25519x; RING_MUL_SYM; PAIR_EQ] THEN
-  RING_TAC);;
-
 let CURVE25519_X25519_BYTE_ALT_CORRECT = time prove
  (`!res scalar n point X pc stackpointer.
     aligned 16 stackpointer /\
     ALL (nonoverlapping (stackpointer,320))
-        [(word pc,0x3de4); (res,32); (scalar,32); (point,32)] /\
-    nonoverlapping (res,32) (word pc,0x3de4)
+        [(word pc,0x3d94); (res,32); (scalar,32); (point,32)] /\
+    nonoverlapping (res,32) (word pc,0x3d94)
     ==> ensures arm
          (\s. aligned_bytes_loaded s (word pc) curve25519_x25519_byte_alt_mc /\
               read PC s = word(pc + 0x10) /\
@@ -4951,7 +5092,7 @@ let CURVE25519_X25519_BYTE_ALT_CORRECT = time prove
               C_ARGUMENTS [res; scalar; point] s /\
               read (memory :> bytes(scalar,32)) s = n /\
               read (memory :> bytes(point,32)) s = X)
-         (\s. read PC s = word (pc + 0x3dd0) /\
+         (\s. read PC s = word (pc + 0x3d80) /\
               read (memory :> bytes(res,32)) s = rfcx25519(n,X))
           (MAYCHANGE [PC; X0; X1; X2; X3; X4; X5; X6; X7; X8; X9; X10;
                       X11; X12; X13; X14; X15; X16; X17; X19; X20;
@@ -4976,7 +5117,7 @@ let CURVE25519_X25519_BYTE_ALT_CORRECT = time prove
   (*** Setup of the main loop ***)
 
   ENSURES_WHILE_ADOWN_TAC `254` `3` `pc + 0x898` `pc + 0x1724`
-   `\i s.
+  `\i s.
       read SP s = stackpointer /\
       read X23 s = res /\
       read X20 s = word_sub (word i) (word 1) /\
@@ -4987,33 +5128,14 @@ let CURVE25519_X25519_BYTE_ALT_CORRECT = time prove
       bignum_from_memory(word_add stackpointer (word 160),4) s < 2 * p_25519 /\
       bignum_from_memory(word_add stackpointer (word 224),4) s < 2 * p_25519 /\
       bignum_from_memory(word_add stackpointer (word 288),4) s < 2 * p_25519 /\
-      !(f:(int#int) ring) P.
-        field f /\ ring_char f = p_25519 /\
-        P IN group_carrier(curve25519x_group f) /\
-        curve25519x_halfcanonically_represents f P (X,1)
-      ==>
-      if X MOD p_25519 = 0 then
-        bignum_from_memory(word_add stackpointer (word 64),4) s
-          MOD p_25519 <= 1 /\
-        bignum_from_memory(word_add stackpointer (word 160),4) s
-          MOD p_25519 = 0 /\
-        bignum_from_memory(word_add stackpointer (word 224),4) s
-          MOD p_25519 = 0 /\
-        bignum_from_memory(word_add stackpointer (word 288),4) s
-          MOD p_25519 <= 1
-      else
-      curve25519x_halfcanonically_represents f
-       (group_pow (curve25519x_group f) P
-           (if ODD(nn DIV 2 EXP i)
-            then nn DIV 2 EXP i + 1 else nn DIV 2 EXP i))
-       (bignum_from_memory(word_add stackpointer (word 288),4) s,
-        bignum_from_memory(word_add stackpointer (word 160),4) s) /\
-      curve25519x_halfcanonically_represents f
-       (group_pow (curve25519x_group f) P
-          (if ODD(nn DIV 2 EXP i)
-           then nn DIV 2 EXP i else nn DIV 2 EXP i + 1))
-       (bignum_from_memory(word_add stackpointer (word 224),4) s,
-        bignum_from_memory(word_add stackpointer (word 64),4) s)` THEN
+      (&(bignum_from_memory(word_add stackpointer (word 288),4) s) ==
+       ladder_x2 X nn i) (mod &p_25519) /\
+      (&(bignum_from_memory(word_add stackpointer (word 160),4) s) ==
+       ladder_z2 X nn i) (mod &p_25519) /\
+      (&(bignum_from_memory(word_add stackpointer (word 224),4) s) ==
+       ladder_x3 X nn i) (mod &p_25519) /\
+      (&(bignum_from_memory(word_add stackpointer (word 64),4) s) ==
+       ladder_z3 X nn i) (mod &p_25519)` THEN
   REPEAT CONJ_TAC THENL
    [ARITH_TAC;
 
@@ -5081,6 +5203,12 @@ let CURVE25519_X25519_BYTE_ALT_CORRECT = time prove
     SUBGOAL_THEN `X < 2 * p_25519` ASSUME_TAC THENL
      [EXPAND_TAC "X" THEN REWRITE_TAC[p_25519] THEN ARITH_TAC;
       ALL_TAC] THEN
+   REWRITE_TAC[ladder_x2; ladder_z2; ladder_x3; ladder_z3] THEN
+    REWRITE_TAC[flipladder; ARITH_RULE `255 - 254 = 0 + 1`] THEN
+    CONV_TAC(ONCE_DEPTH_CONV let_CONV) THEN
+    REWRITE_TAC[SUB_0; ADD_CLAUSES; ARITH_RULE `255 - 1 = 254`] THEN
+    SUBGOAL_THEN `nn DIV 2 EXP 255 = 0` SUBST1_TAC THENL
+     [EXPAND_TAC "nn" THEN ARITH_TAC; ALL_TAC] THEN
     SUBGOAL_THEN `nn DIV 2 EXP 254 = 1` SUBST1_TAC THENL
      [EXPAND_TAC "nn" THEN SIMP_TAC[DIV_ADD; DIVIDES_REFL] THEN
       SIMP_TAC[DIV_LT; ARITH_RULE `x:num < n ==> x - k < n`;
@@ -5089,11 +5217,11 @@ let CURVE25519_X25519_BYTE_ALT_CORRECT = time prove
       CONV_TAC(DEPTH_CONV WORD_NUM_RED_CONV)] THEN
     ASM_REWRITE_TAC[] THEN
     CONJ_TAC THENL [REWRITE_TAC[p_25519] THEN ARITH_TAC; ALL_TAC] THEN
-    SIMP_TAC[GROUP_POW_1] THEN
-    REPEAT(FIRST_X_ASSUM(K ALL_TAC o SYM)) THEN
-    ASM_REWRITE_TAC[curve25519x_halfcanonically_represents] THEN
+    REWRITE_TAC[INT_CONG_REFL] THEN
+    REWRITE_TAC[montgomery_xzdouble; curve25519; A_25519] THEN
+    REWRITE_TAC[INTEGER_MOD_RING_CLAUSES] THEN
     REPEAT(FIRST_X_ASSUM(MP_TAC o check (is_imp o concl))) THEN
-    ASM_REWRITE_TAC[] THEN
+    ASM_REWRITE_TAC[GSYM INT_REM_EQ] THEN
     REPEAT
      (ANTS_TAC THENL [REWRITE_TAC[p_25519] THEN ARITH_TAC; STRIP_TAC]) THEN
     STRIP_TAC THEN
@@ -5103,29 +5231,8 @@ let CURVE25519_X25519_BYTE_ALT_CORRECT = time prove
     RULE_ASSUM_TAC(REWRITE_RULE[GSYM INT_REM_EQ]) THEN
     RULE_ASSUM_TAC(ONCE_REWRITE_RULE[GSYM INT_SUB_REM; GSYM INT_ADD_REM]) THEN
     RULE_ASSUM_TAC(ONCE_REWRITE_RULE[GSYM INT_POW_REM; GSYM INT_MUL_REM]) THEN
-    ONCE_REWRITE_TAC[GSYM RING_OF_INT_OF_NUM] THEN
-    ONCE_REWRITE_TAC[GSYM RING_OF_INT_REM] THEN
-    MAP_EVERY X_GEN_TAC
-     [`f:(int#int) ring`; `P:((int#int)#(int#int))option`] THEN
-    REPEAT(DISCH_THEN(CONJUNCTS_THEN2 ASSUME_TAC MP_TAC)) THEN
-    ASM_REWRITE_TAC[GSYM INT_OF_NUM_REM; GSYM INT_OF_NUM_CLAUSES] THEN
-    SIMP_TAC[] THEN CONV_TAC INT_REM_DOWN_CONV THEN
-    COND_CASES_TAC THEN ASM_REWRITE_TAC[] THENL
-     [DISCH_THEN(K ALL_TAC) THEN REWRITE_TAC[p_25519] THEN
-      CONV_TAC INT_REDUCE_CONV;
-      ALL_TAC] THEN
-    DISCH_THEN(MP_TAC o MATCH_MP (ONCE_REWRITE_RULE[IMP_CONJ_ALT]
-        lemma_double_base)) THEN
-    ASM_REWRITE_TAC[] THEN
-    MATCH_MP_TAC EQ_IMP THEN AP_TERM_TAC THEN
-    ASM_REWRITE_TAC[montgomery_xzdouble; curve25519x; PAIR_EQ] THEN
-    REWRITE_TAC[GSYM RING_OF_INT_OF_NUM; RING_OF_INT_CLAUSES] THEN
-    ASM_REWRITE_TAC[RING_OF_INT_EQ] THEN
-    REWRITE_TAC[GSYM INT_OF_NUM_REM; GSYM INT_REM_EQ;
-                GSYM INT_OF_NUM_CLAUSES] THEN
-    CONV_TAC INT_REM_DOWN_CONV THEN
-    REPEAT CONJ_TAC THEN AP_THM_TAC THEN AP_TERM_TAC THEN
-    REWRITE_TAC[A_25519] THEN INT_ARITH_TAC;
+    ASM_REWRITE_TAC[] THEN CONV_TAC INT_REM_DOWN_CONV THEN
+    REPEAT CONJ_TAC THEN AP_THM_TAC THEN AP_TERM_TAC THEN INT_ARITH_TAC;
 
     (*** The main loop invariant for the Montgomery ladder ***)
 
@@ -5223,90 +5330,33 @@ let CURVE25519_X25519_BYTE_ALT_CORRECT = time prove
     DISCARD_STATE_TAC "s28" THEN
     DISCARD_MATCHING_ASSUMPTIONS
      [`aligned a b`; `val(word i) = i`; `nonoverlapping_modulo a b c`] THEN
+    REWRITE_TAC[ladder_x2; ladder_z2; ladder_x3; ladder_z3] THEN
+    ASM_SIMP_TAC[ARITH_RULE `i < 254 ==> 255 - i = (255 - (i + 1)) + 1`] THEN
+    REWRITE_TAC[flipladder] THEN
+    ASM_SIMP_TAC[ARITH_RULE `i < 254 ==> ~(255 - (i + 1) = 0)`] THEN
+    ASM_SIMP_TAC[ARITH_RULE `i < 254 ==> 255 - (255 - (i + 1)) = i + 1`] THEN
+    ASM_SIMP_TAC[ARITH_RULE `i < 254 ==> 255 - (255 - (i + 1) + 1) = i`] THEN
+    RULE_ASSUM_TAC(REWRITE_RULE
+      [ladder_x2; ladder_z2; ladder_x3; ladder_z3]) THEN
+    LET_TAC THEN RULE_ASSUM_TAC(REWRITE_RULE[]) THEN
+    CONV_TAC(ONCE_DEPTH_CONV let_CONV) THEN
+    REPEAT(FIRST_X_ASSUM(MP_TAC o check (is_imp o concl))) THEN
+    ASM_REWRITE_TAC[GSYM INT_REM_EQ] THEN
+    REPEAT
+     (ANTS_TAC THENL [REWRITE_TAC[p_25519] THEN ARITH_TAC; STRIP_TAC]) THEN
+    POP_ASSUM_LIST(MP_TAC o end_itlist CONJ o rev) THEN
+    REWRITE_TAC[ISPEC `p:bool` EQ_SYM_EQ] THEN
+    COND_CASES_TAC THEN ASM_REWRITE_TAC[] THEN STRIP_TAC THEN
     RULE_ASSUM_TAC(REWRITE_RULE[EXP_2]) THEN
     RULE_ASSUM_TAC(REWRITE_RULE[num_congruent; GSYM INT_OF_NUM_CLAUSES]) THEN
     RULE_ASSUM_TAC(REWRITE_RULE[GSYM INT_REM_EQ]) THEN
     RULE_ASSUM_TAC(ONCE_REWRITE_RULE[GSYM INT_SUB_REM; GSYM INT_ADD_REM]) THEN
     RULE_ASSUM_TAC(ONCE_REWRITE_RULE[GSYM INT_POW_REM; GSYM INT_MUL_REM]) THEN
-    MAP_EVERY X_GEN_TAC
-     [`f:(int#int) ring`; `P:((int#int)#(int#int))option`] THEN
-    STRIP_TAC THEN FIRST_X_ASSUM(MP_TAC o SPECL
-    [`f:(int#int) ring`; `P:((int#int)#(int#int))option`]) THEN
-    ASM_REWRITE_TAC[] THEN
-    REWRITE_TAC[GSYM INT_OF_NUM_CLAUSES; GSYM INT_OF_NUM_REM] THEN
-    COND_CASES_TAC THEN ASM_REWRITE_TAC[] THENL
-     [REWRITE_TAC[INT_OF_NUM_CLAUSES; INT_OF_NUM_REM] THEN
-      REWRITE_TAC[ARITH_RULE `b <= 1 <=> b = 0 \/ b = 1`] THEN
-      REWRITE_TAC[GSYM INT_OF_NUM_CLAUSES; GSYM INT_OF_NUM_REM] THEN
-      STRIP_TAC THEN ASM_REWRITE_TAC[] THEN
-      COND_CASES_TAC THEN ASM_REWRITE_TAC[] THEN
-      CONV_TAC INT_REM_DOWN_CONV THEN
-      REWRITE_TAC[p_25519] THEN CONV_TAC INT_REDUCE_CONV;
-      ALL_TAC] THEN
-    RULE_ASSUM_TAC(ONCE_REWRITE_RULE[TAUT
-     `(ODD n <=> b) <=> (b <=> ODD n)`]) THEN
-    ABBREV_TAC `n = nn DIV 2 EXP (i + 1)` THEN
-    ABBREV_TAC `b = ODD(nn DIV 2 EXP i)` THEN
-    SUBGOAL_THEN `nn DIV 2 EXP i = 2 * n + bitval b` SUBST1_TAC THENL
-     [MAP_EVERY EXPAND_TAC ["b"; "n"] THEN
-      REWRITE_TAC[EXP_ADD; GSYM DIV_DIV; BITVAL_ODD] THEN ARITH_TAC;
-      SIMP_TAC[BITVAL_CLAUSES; ADD_CLAUSES; COND_ID]] THEN
-    DISCH_TAC THEN
-    SUBGOAL_THEN
-     `(ring_of_num f xm':(int#int),ring_of_num f zm') =
-       montgomery_xzdiffadd (curve25519x f)
-           (ring_of_num f X,ring_of_num f 1)
-           (ring_of_num f xn,ring_of_num f zn)
-           (ring_of_num f xm,ring_of_num f zm) /\
-      (ring_of_num f xn',ring_of_num f zn') =
-       montgomery_xzdouble (curve25519x f)
-        (if b <=> ODD n then (ring_of_num f xn,ring_of_num f zn)
-         else (ring_of_num f xm,ring_of_num f zm))`
-    MP_TAC THENL
-     [COND_CASES_TAC THEN
-      ASM_REWRITE_TAC[montgomery_xzdiffadd; montgomery_xzdouble;
-                      curve25519x; PAIR_EQ] THEN
-      REWRITE_TAC[GSYM RING_OF_INT_OF_NUM; RING_OF_INT_CLAUSES] THEN
-      ASM_REWRITE_TAC[RING_OF_INT_EQ] THEN
-      REWRITE_TAC[GSYM INT_OF_NUM_REM; GSYM INT_REM_EQ;
-                  GSYM INT_OF_NUM_CLAUSES] THEN
-      CONV_TAC INT_REM_DOWN_CONV THEN
-      ASM_REWRITE_TAC[] THEN CONV_TAC INT_REM_DOWN_CONV THEN
-      REPEAT CONJ_TAC THEN AP_THM_TAC THEN AP_TERM_TAC THEN
-      REWRITE_TAC[A_25519] THEN INT_ARITH_TAC;
-      ASM_REWRITE_TAC[] THEN
-      SIMP_TAC[curve25519x_halfcanonically_represents] THEN
-      DISCH_THEN(K ALL_TAC) THEN
-      ASM_REWRITE_TAC[GSYM INT_OF_NUM_CLAUSES] THEN
-      FIRST_X_ASSUM(CONJUNCTS_THEN(MP_TAC o last o CONJUNCTS o
-        GEN_REWRITE_RULE I [curve25519x_halfcanonically_represents])) THEN
-      GEN_REWRITE_TAC I [GSYM IMP_CONJ_ALT] THEN
-      FIRST_X_ASSUM(MP_TAC o GEN_REWRITE_RULE I
-       [curve25519x_halfcanonically_represents]) THEN
-     DISCH_THEN(CONJUNCTS_THEN2 ASSUME_TAC (MP_TAC o CONJUNCT2)) THEN
-      UNDISCH_TAC
-       `P IN group_carrier(curve25519x_group(f:(int#int) ring))`] THEN
-    SUBGOAL_THEN `~(ring_of_num (f:(int#int) ring) X = ring_0 f)` MP_TAC THENL
-     [ASM_REWRITE_TAC[RING_OF_NUM_EQ_0; DIVIDES_MOD] THEN
-      ASM_REWRITE_TAC[GSYM INT_OF_NUM_CLAUSES; GSYM INT_OF_NUM_REM];
-      MAP_EVERY UNDISCH_TAC
-       [`ring_char(f:(int#int) ring) = p_25519`; `field(f:(int#int) ring)`] THEN
-      POP_ASSUM_LIST(K ALL_TAC)] THEN
-    REPEAT DISCH_TAC THEN CONJ_TAC THENL
-     [DISJ_CASES_THEN SUBST_ALL_TAC
-       (TAUT `(b <=> ODD n) \/ (b <=> ~ODD n)`) THEN
-      REWRITE_TAC[TAUT `~(~p <=> p)`] THENL
-       [FIRST_X_ASSUM(MP_TAC o CONJUNCT1);
-        FIRST_X_ASSUM(MP_TAC o CONJUNCT2)] THEN
-      UNDISCH_TAC `P IN group_carrier(curve25519x_group(f:(int#int) ring))` THEN
-      REWRITE_TAC[IMP_IMP] THEN DISCH_THEN(MP_TAC o MATCH_MP lemma_double) THEN
-      ASM_REWRITE_TAC[COND_SWAP] THEN COND_CASES_TAC THEN
-      REWRITE_TAC[ARITH_RULE `(2 * n + 1) + 1 = 2 * (n + 1)`];
-      REPEAT(POP_ASSUM MP_TAC) THEN
-      REWRITE_TAC[IMP_IMP; GSYM CONJ_ASSOC] THEN
-      COND_CASES_TAC THEN REWRITE_TAC[lemma_diffadd1] THEN
-      GEN_REWRITE_TAC (LAND_CONV o funpow 5 RAND_CONV) [CONJ_SYM] THEN
-      REWRITE_TAC[lemma_diffadd2]];
+    ASM_REWRITE_TAC[GSYM INT_REM_EQ] THEN CONV_TAC INT_REM_DOWN_CONV THEN
+    ASM_REWRITE_TAC[montgomery_xzdouble; montgomery_xzdiffadd;
+                    curve25519; A_25519; INTEGER_MOD_RING_CLAUSES] THEN
+    CONV_TAC INT_REM_DOWN_CONV THEN
+    REPEAT CONJ_TAC THEN AP_THM_TAC THEN AP_TERM_TAC THEN INT_ARITH_TAC;
 
     (*** The trivial loop-back subgoal ***)
 
@@ -5333,43 +5383,8 @@ let CURVE25519_X25519_BYTE_ALT_CORRECT = time prove
   REWRITE_TAC(!simulation_precanon_thms) THEN ENSURES_INIT_TAC "s0" THEN
   LOCAL_MUX_4_TAC 3 ["xn"; "xm"; "xn"] THEN
   LOCAL_MUX_4_TAC 0 ["zn"; "zm"; "zn"] THEN
-
-  MAP_EVERY (fun t -> REABBREV_TAC t THEN POP_ASSUM SUBST_ALL_TAC)
-   [`xn8 = read(memory :> bytes(word_add stackpointer (word 288),8 * 4)) s5`;
-    `zn8 =
-     read(memory :> bytes(word_add stackpointer (word 160),8 * 4)) s5`] THEN
-  SUBGOAL_THEN
-   `xn8 < 2 * p_25519 /\ zn8 < 2 * p_25519 /\
-     !(f:(int#int) ring) P.
-        field f /\ ring_char f = p_25519 /\
-        P IN group_carrier(curve25519x_group f) /\
-        curve25519x_halfcanonically_represents f P (X,1)
-      ==>
-      if X MOD p_25519 = 0 then
-        xn8 MOD p_25519 = 0 /\ zn8 MOD p_25519 <= 1 \/
-        xn8 MOD p_25519 <= 1 /\ zn8 MOD p_25519 = 0
-      else
-      curve25519x_halfcanonically_represents f
-       (group_pow (curve25519x_group f) P (nn DIV 8)) (xn8,zn8)`
-  MP_TAC THENL
-   [ASM_REWRITE_TAC[VAL_WORD_BITVAL; BITVAL_EQ_0; COND_SWAP] THEN
-    REPLICATE_TAC 2
-     (CONJ_TAC THENL [COND_CASES_TAC THEN ASM_REWRITE_TAC[]; ALL_TAC]) THEN
-    MAP_EVERY X_GEN_TAC
-     [`f:(int#int) ring`; `P:((int#int)#(int#int))option`] THEN
-    STRIP_TAC THEN FIRST_X_ASSUM(MP_TAC o SPECL
-    [`f:(int#int) ring`; `P:((int#int)#(int#int))option`]) THEN
-    ASM_REWRITE_TAC[] THEN
-    REWRITE_TAC[VAL_EQ_0; WORD_SUB_EQ_0; WORD_BITVAL_EQ_0] THEN
-    COND_CASES_TAC THEN ASM_REWRITE_TAC[] THENL [ARITH_TAC; ALL_TAC] THEN
-    REWRITE_TAC[NUM_REDUCE_CONV `2 EXP 3`] THEN
-    COND_CASES_TAC THEN ASM_SIMP_TAC[];
-
-    FIRST_X_ASSUM(K ALL_TAC o check (is_forall o concl)) THEN
-    REPEAT(FIRST_X_ASSUM(K ALL_TAC o check
-     (fun th -> intersect (frees (concl th))
-                [`xm:num`; `xn:num`; `zm:num`; `zn:num`] <> []))) THEN
-    STRIP_TAC] THEN
+  RULE_ASSUM_TAC(REWRITE_RULE
+   [WORD_SUB_0; VAL_WORD_BITVAL; BITVAL_EQ_0; COND_SWAP]) THEN
 
   (*** The first doubling to get from nn/8 to nn/4 ***)
 
@@ -5385,59 +5400,47 @@ let CURVE25519_X25519_BYTE_ALT_CORRECT = time prove
    [`xn4 = read(memory :> bytes(word_add stackpointer (word 288),8 * 4)) s15`;
     `zn4 =
      read(memory :> bytes(word_add stackpointer (word 160),8 * 4)) s15`] THEN
+  SUBGOAL_THEN `8 divides nn` ASSUME_TAC THENL
+   [EXPAND_TAC "nn" THEN REWRITE_TAC[DIVIDES_MOD] THEN
+    REWRITE_TAC[ARITH_RULE `2 EXP 254 = 8 * 2 EXP 251`; MOD_MULT_MOD] THEN
+    REWRITE_TAC[ADD_SUB; GSYM LEFT_ADD_DISTRIB; MOD_MULT];
+    ALL_TAC] THEN
   SUBGOAL_THEN
-   `xn4 < 2 * p_25519 /\ zn4 < 2 * p_25519 /\
-     !(f:(int#int) ring) P.
-        field f /\ ring_char f = p_25519 /\
-        P IN group_carrier(curve25519x_group f) /\
-        curve25519x_halfcanonically_represents f P (X,1)
-      ==>
-      if X MOD p_25519 = 0 then
-        xn4 MOD p_25519 = 0 /\ zn4 MOD p_25519 <= 1 \/
-        xn4 MOD p_25519 <= 1 /\ zn4 MOD p_25519 = 0
-      else
-      curve25519x_halfcanonically_represents f
-       (group_pow (curve25519x_group f) P (2 * nn DIV 8)) (xn4,zn4)`
+   `(&xn4 == ladder_x2 X nn 2) (mod &p_25519) /\
+    (&zn4 == ladder_z2 X nn 2) (mod &p_25519)`
   MP_TAC THENL
-   [ASM_REWRITE_TAC[] THEN
-    MAP_EVERY X_GEN_TAC
-     [`f:(int#int) ring`; `P:((int#int)#(int#int))option`] THEN
-    STRIP_TAC THEN FIRST_X_ASSUM(MP_TAC o SPECL
-    [`f:(int#int) ring`; `P:((int#int)#(int#int))option`]) THEN
-    ASM_REWRITE_TAC[] THEN
-    COND_CASES_TAC THEN ASM_REWRITE_TAC[] THEN
+   [REWRITE_TAC[ladder_x2; ladder_z2; ladder_x3; ladder_z3] THEN
+    REWRITE_TAC[ARITH_RULE `255 - 2 = (255 - 3) + 1`; flipladder] THEN
+    RULE_ASSUM_TAC(REWRITE_RULE
+     [ladder_x2; ladder_z2; ladder_x3; ladder_z3]) THEN
+    LET_TAC THEN CONV_TAC(ONCE_DEPTH_CONV let_CONV) THEN
+    RULE_ASSUM_TAC(REWRITE_RULE[]) THEN CONV_TAC NUM_REDUCE_CONV THEN
+    SUBGOAL_THEN `ODD(nn DIV 4) <=> F` SUBST_ALL_TAC THENL
+     [REWRITE_TAC[NOT_ODD; GSYM DIVIDES_2] THEN
+      MATCH_MP_TAC DIVIDES_DIVIDES_DIV_IMP THEN ASM_REWRITE_TAC[ARITH];
+      ALL_TAC] THEN
+    POP_ASSUM_LIST(MP_TAC o end_itlist CONJ o rev) THEN
+    REWRITE_TAC[] THEN COND_CASES_TAC THEN
+    ASM_REWRITE_TAC[] THEN STRIP_TAC THEN
+    REPEAT(FIRST_X_ASSUM(MP_TAC o check (is_imp o concl))) THEN
+    ASM_REWRITE_TAC[GSYM INT_REM_EQ] THEN
+    REPEAT
+     (ANTS_TAC THENL [REWRITE_TAC[p_25519] THEN ARITH_TAC; STRIP_TAC]) THEN
+    REPEAT DISCH_TAC THEN
     RULE_ASSUM_TAC(REWRITE_RULE[EXP_2]) THEN
     RULE_ASSUM_TAC(REWRITE_RULE[num_congruent; GSYM INT_OF_NUM_CLAUSES]) THEN
-    RULE_ASSUM_TAC(REWRITE_RULE[GSYM INT_OF_NUM_REM; GSYM INT_REM_EQ]) THEN
+    RULE_ASSUM_TAC(REWRITE_RULE[GSYM INT_REM_EQ]) THEN
     RULE_ASSUM_TAC(ONCE_REWRITE_RULE[GSYM INT_SUB_REM; GSYM INT_ADD_REM]) THEN
-    RULE_ASSUM_TAC(ONCE_REWRITE_RULE[GSYM INT_POW_REM; GSYM INT_MUL_REM]) THENL
-     [REWRITE_TAC[ARITH_RULE `n <= 1 <=> n = 0 \/ n = 1`] THEN
-      ASM_REWRITE_TAC[GSYM INT_OF_NUM_CLAUSES; GSYM INT_OF_NUM_REM] THEN
-      STRIP_TAC THEN ASM_REWRITE_TAC[] THEN
-      REWRITE_TAC[p_25519] THEN CONV_TAC INT_REDUCE_CONV;
-      ALL_TAC] THEN
-    REWRITE_TAC[curve25519x_halfcanonically_represents] THEN
-    ASM_REWRITE_TAC[GSYM INT_OF_NUM_CLAUSES] THEN
-    DISCH_THEN(MP_TAC o MATCH_MP (ONCE_REWRITE_RULE[IMP_CONJ_ALT]
-        lemma_double)) THEN
-    ASM_REWRITE_TAC[GSYM INT_OF_NUM_EQ] THEN MATCH_MP_TAC EQ_IMP THEN
-    AP_TERM_TAC THEN REWRITE_TAC[PAIR_EQ] THEN
-    ONCE_REWRITE_TAC[GSYM RING_OF_INT_OF_NUM] THEN
-    ONCE_REWRITE_TAC[GSYM RING_OF_INT_REM] THEN
-    ASM_REWRITE_TAC[] THEN
-    ASM_REWRITE_TAC[montgomery_xzdouble; curve25519x; PAIR_EQ] THEN
-    REWRITE_TAC[GSYM RING_OF_INT_OF_NUM; RING_OF_INT_CLAUSES] THEN
-    ASM_REWRITE_TAC[RING_OF_INT_EQ] THEN
-    REWRITE_TAC[GSYM INT_OF_NUM_REM; GSYM INT_REM_EQ;
-                GSYM INT_OF_NUM_CLAUSES] THEN
+    RULE_ASSUM_TAC(ONCE_REWRITE_RULE[GSYM INT_POW_REM; GSYM INT_MUL_REM]) THEN
+    ASM_REWRITE_TAC[GSYM INT_REM_EQ] THEN CONV_TAC INT_REM_DOWN_CONV THEN
+    ASM_REWRITE_TAC[montgomery_xzdouble; montgomery_xzdiffadd;
+                    curve25519; A_25519; INTEGER_MOD_RING_CLAUSES] THEN
     CONV_TAC INT_REM_DOWN_CONV THEN
-    REPEAT CONJ_TAC THEN AP_THM_TAC THEN AP_TERM_TAC THEN
-    REWRITE_TAC[A_25519] THEN INT_ARITH_TAC;
-
-    FIRST_X_ASSUM(K ALL_TAC o check (is_forall o concl)) THEN
+    REPEAT CONJ_TAC THEN AP_THM_TAC THEN AP_TERM_TAC THEN INT_ARITH_TAC;
     REPEAT(FIRST_X_ASSUM(K ALL_TAC o check
      (fun th -> intersect (frees (concl th))
-                [`xn8:num`; `zn8:num`; `d:num`; `d':num`;
+                [`xn:num`; `zn:num`; `xm:num`; `zm:num`;
+                 `xn':num`; `zn':num`; `d:num`; `d':num`;
                  `s:num`; `s':num`; `p:num`; `e:num`] <> []))) THEN
     STRIP_TAC] THEN
 
@@ -5456,58 +5459,34 @@ let CURVE25519_X25519_BYTE_ALT_CORRECT = time prove
     `zn2 =
      read(memory :> bytes(word_add stackpointer (word 160),8 * 4)) s25`] THEN
   SUBGOAL_THEN
-   `xn2 < 2 * p_25519 /\ zn2 < 2 * p_25519 /\
-     !(f:(int#int) ring) P.
-        field f /\ ring_char f = p_25519 /\
-        P IN group_carrier(curve25519x_group f) /\
-        curve25519x_halfcanonically_represents f P (X,1)
-      ==>
-      if X MOD p_25519 = 0 then
-        xn2 MOD p_25519 = 0 /\ zn2 MOD p_25519 <= 1 \/
-        xn2 MOD p_25519 <= 1 /\ zn2 MOD p_25519 = 0
-      else
-      curve25519x_halfcanonically_represents f
-       (group_pow (curve25519x_group f) P (2 * 2 * nn DIV 8)) (xn2,zn2)`
+   `(&xn2 == ladder_x2 X nn 1) (mod &p_25519) /\
+    (&zn2 == ladder_z2 X nn 1) (mod &p_25519)`
   MP_TAC THENL
-   [ASM_REWRITE_TAC[] THEN
-    MAP_EVERY X_GEN_TAC
-     [`f:(int#int) ring`; `P:((int#int)#(int#int))option`] THEN
-    STRIP_TAC THEN FIRST_X_ASSUM(MP_TAC o SPECL
-    [`f:(int#int) ring`; `P:((int#int)#(int#int))option`]) THEN
-    ASM_REWRITE_TAC[] THEN
-    COND_CASES_TAC THEN ASM_REWRITE_TAC[] THEN
+   [REWRITE_TAC[ladder_x2; ladder_z2; ladder_x3; ladder_z3] THEN
+    REWRITE_TAC[ARITH_RULE `255 - 1 = (255 - 2) + 1`; flipladder] THEN
+    RULE_ASSUM_TAC(REWRITE_RULE
+     [ladder_x2; ladder_z2; ladder_x3; ladder_z3]) THEN
+    LET_TAC THEN CONV_TAC(ONCE_DEPTH_CONV let_CONV) THEN
+    RULE_ASSUM_TAC(REWRITE_RULE[]) THEN CONV_TAC NUM_REDUCE_CONV THEN
+    SUBGOAL_THEN `nn = 8 * nn DIV 8` SUBST1_TAC THENL
+     [REWRITE_TAC[ARITH_RULE `n = 8 * n DIV 8 <=> n MOD 8 = 0`] THEN
+      ASM_REWRITE_TAC[GSYM DIVIDES_MOD];
+      REWRITE_TAC[ARITH_RULE `(8 * n) DIV 2 = 2 * 2 * n`] THEN
+      REWRITE_TAC[ARITH_RULE `(8 * n) DIV 4 = 2 * n`] THEN
+      REWRITE_TAC[ODD_MULT; ARITH_ODD; ARITH_EVEN]] THEN
     RULE_ASSUM_TAC(REWRITE_RULE[EXP_2]) THEN
     RULE_ASSUM_TAC(REWRITE_RULE[num_congruent; GSYM INT_OF_NUM_CLAUSES]) THEN
-    RULE_ASSUM_TAC(REWRITE_RULE[GSYM INT_OF_NUM_REM; GSYM INT_REM_EQ]) THEN
+    RULE_ASSUM_TAC(REWRITE_RULE[GSYM INT_REM_EQ]) THEN
     RULE_ASSUM_TAC(ONCE_REWRITE_RULE[GSYM INT_SUB_REM; GSYM INT_ADD_REM]) THEN
-    RULE_ASSUM_TAC(ONCE_REWRITE_RULE[GSYM INT_POW_REM; GSYM INT_MUL_REM]) THENL
-     [REWRITE_TAC[ARITH_RULE `n <= 1 <=> n = 0 \/ n = 1`] THEN
-      ASM_REWRITE_TAC[GSYM INT_OF_NUM_CLAUSES; GSYM INT_OF_NUM_REM] THEN
-      STRIP_TAC THEN ASM_REWRITE_TAC[] THEN
-      REWRITE_TAC[p_25519] THEN CONV_TAC INT_REDUCE_CONV;
-      ALL_TAC] THEN
-    REWRITE_TAC[curve25519x_halfcanonically_represents] THEN
-    ASM_REWRITE_TAC[GSYM INT_OF_NUM_CLAUSES] THEN
-    DISCH_THEN(MP_TAC o MATCH_MP (ONCE_REWRITE_RULE[IMP_CONJ_ALT]
-        lemma_double)) THEN
-    ASM_REWRITE_TAC[GSYM INT_OF_NUM_EQ] THEN MATCH_MP_TAC EQ_IMP THEN
-    AP_TERM_TAC THEN REWRITE_TAC[PAIR_EQ] THEN
-    ONCE_REWRITE_TAC[GSYM RING_OF_INT_OF_NUM] THEN
-    ONCE_REWRITE_TAC[GSYM RING_OF_INT_REM] THEN
-    ASM_REWRITE_TAC[] THEN
-    ASM_REWRITE_TAC[montgomery_xzdouble; curve25519x; PAIR_EQ] THEN
-    REWRITE_TAC[GSYM RING_OF_INT_OF_NUM; RING_OF_INT_CLAUSES] THEN
-    ASM_REWRITE_TAC[RING_OF_INT_EQ] THEN
-    REWRITE_TAC[GSYM INT_OF_NUM_REM; GSYM INT_REM_EQ;
-                GSYM INT_OF_NUM_CLAUSES] THEN
+    RULE_ASSUM_TAC(ONCE_REWRITE_RULE[GSYM INT_POW_REM; GSYM INT_MUL_REM]) THEN
+    ASM_REWRITE_TAC[GSYM INT_REM_EQ] THEN CONV_TAC INT_REM_DOWN_CONV THEN
+    ASM_REWRITE_TAC[montgomery_xzdouble; montgomery_xzdiffadd;
+                    curve25519; A_25519; INTEGER_MOD_RING_CLAUSES] THEN
     CONV_TAC INT_REM_DOWN_CONV THEN
-    REPEAT CONJ_TAC THEN AP_THM_TAC THEN AP_TERM_TAC THEN
-    REWRITE_TAC[A_25519] THEN INT_ARITH_TAC;
-
-    FIRST_X_ASSUM(K ALL_TAC o check (is_forall o concl)) THEN
+    REPEAT CONJ_TAC THEN AP_THM_TAC THEN AP_TERM_TAC THEN INT_ARITH_TAC;
     REPEAT(FIRST_X_ASSUM(K ALL_TAC o check
      (fun th -> intersect (frees (concl th))
-                [`xn4:num`; `zn4:num`; `d:num`; `d':num`;
+                [`xn4:num`; `zn4:num`;  `d:num`; `d':num`;
                  `s:num`; `s':num`; `p:num`; `e:num`] <> []))) THEN
     STRIP_TAC] THEN
 
@@ -5520,136 +5499,55 @@ let CURVE25519_X25519_BYTE_ALT_CORRECT = time prove
   LOCAL_SUB_TWICE4_TAC 0 ["p"; "s"; "d"] THEN
   LOCAL_CMADD_4_TAC 2 ["e"; "p"; "d"] THEN
   LOCAL_MUL_4_TAC 0 ["xn"; "s"; "d"] THEN
-  LOCAL_MUL_P25519_TAC 0 ["zn"; "p"; "e"] THEN
+  LOCAL_MUL_4_TAC 0 ["zn"; "p"; "e"] THEN
   SUBGOAL_THEN
-   `xn < 2 * p_25519 /\ zn < p_25519 /\
-     !(f:(int#int) ring) P.
-        field f /\ ring_char f = p_25519 /\
-        P IN group_carrier(curve25519x_group f) /\
-        curve25519x_halfcanonically_represents f P (X,1)
-      ==>
-      if X MOD p_25519 = 0 then
-        xn MOD p_25519 = 0 /\ zn MOD p_25519 <= 1 \/
-        xn MOD p_25519 <= 1 /\ zn MOD p_25519 = 0
-      else
-      curve25519x_halfcanonically_represents f
-       (group_pow (curve25519x_group f) P (2 * 2 * 2 * nn DIV 8)) (xn,zn)`
+   `(&xn == ladder_x2 X nn 0) (mod &p_25519) /\
+    (&zn == ladder_z2 X nn 0) (mod &p_25519)`
   MP_TAC THENL
-   [ASM_REWRITE_TAC[] THEN CONJ_TAC THENL
-     [REWRITE_TAC[MOD_LT_EQ; p_25519; ARITH_EQ]; ALL_TAC] THEN
-    MAP_EVERY X_GEN_TAC
-     [`f:(int#int) ring`; `P:((int#int)#(int#int))option`] THEN
-    STRIP_TAC THEN FIRST_X_ASSUM(MP_TAC o SPECL
-    [`f:(int#int) ring`; `P:((int#int)#(int#int))option`]) THEN
-    ASM_REWRITE_TAC[] THEN
-    COND_CASES_TAC THEN ASM_REWRITE_TAC[] THEN
+   [REWRITE_TAC[ladder_x2; ladder_z2; ladder_x3; ladder_z3] THEN
+    REWRITE_TAC[ARITH_RULE `255 - 0 = (255 - 1) + 1`; flipladder] THEN
+    RULE_ASSUM_TAC(REWRITE_RULE
+     [ladder_x2; ladder_z2; ladder_x3; ladder_z3]) THEN
+    LET_TAC THEN CONV_TAC(ONCE_DEPTH_CONV let_CONV) THEN
+    RULE_ASSUM_TAC(REWRITE_RULE[]) THEN CONV_TAC NUM_REDUCE_CONV THEN
+    SUBGOAL_THEN `nn = 8 * nn DIV 8` SUBST1_TAC THENL
+     [REWRITE_TAC[ARITH_RULE `n = 8 * n DIV 8 <=> n MOD 8 = 0`] THEN
+      ASM_REWRITE_TAC[GSYM DIVIDES_MOD];
+      REWRITE_TAC[ARITH_RULE `(8 * n) DIV 2 = 2 * 2 * n`] THEN
+      REWRITE_TAC[ODD_MULT; ARITH_ODD; ARITH_EVEN; DIV_1]] THEN
     RULE_ASSUM_TAC(REWRITE_RULE[EXP_2]) THEN
     RULE_ASSUM_TAC(REWRITE_RULE[num_congruent; GSYM INT_OF_NUM_CLAUSES]) THEN
-    RULE_ASSUM_TAC(REWRITE_RULE[GSYM INT_OF_NUM_REM; GSYM INT_REM_EQ]) THEN
-    RULE_ASSUM_TAC(REWRITE_RULE[GSYM INT_OF_NUM_CLAUSES]) THEN
+    RULE_ASSUM_TAC(REWRITE_RULE[GSYM INT_REM_EQ]) THEN
     RULE_ASSUM_TAC(ONCE_REWRITE_RULE[GSYM INT_SUB_REM; GSYM INT_ADD_REM]) THEN
     RULE_ASSUM_TAC(ONCE_REWRITE_RULE[GSYM INT_POW_REM; GSYM INT_MUL_REM]) THEN
-    ONCE_REWRITE_TAC[GSYM MOD_MULT_MOD2] THENL
-     [REWRITE_TAC[ARITH_RULE `n <= 1 <=> n = 0 \/ n = 1`] THEN
-      ASM_REWRITE_TAC[GSYM INT_OF_NUM_CLAUSES; GSYM INT_OF_NUM_REM] THEN
-      STRIP_TAC THEN ASM_REWRITE_TAC[] THEN
-      REWRITE_TAC[p_25519] THEN CONV_TAC INT_REDUCE_CONV;
-      ALL_TAC] THEN
-    REWRITE_TAC[curve25519x_halfcanonically_represents] THEN
-    ASM_REWRITE_TAC[GSYM INT_OF_NUM_CLAUSES] THEN
-    MATCH_MP_TAC(TAUT `q /\ (p ==> r) ==> p ==> q /\ r`) THEN
-    CONJ_TAC THENL
-     [REWRITE_TAC[INT_OF_NUM_CLAUSES] THEN
-      MATCH_MP_TAC(ARITH_RULE `x < p ==> x < 2 * p`) THEN
-      REWRITE_TAC[MOD_LT_EQ; p_25519; ARITH_EQ];
-      ALL_TAC] THEN
-    DISCH_THEN(MP_TAC o MATCH_MP (ONCE_REWRITE_RULE[IMP_CONJ_ALT]
-        lemma_double)) THEN
-    ASM_REWRITE_TAC[GSYM INT_OF_NUM_EQ] THEN MATCH_MP_TAC EQ_IMP THEN
-    AP_TERM_TAC THEN REWRITE_TAC[PAIR_EQ] THEN
-    ONCE_REWRITE_TAC[GSYM RING_OF_INT_OF_NUM] THEN
-    ONCE_REWRITE_TAC[GSYM RING_OF_INT_REM] THEN
-    ASM_REWRITE_TAC[] THEN
-    ASM_REWRITE_TAC[montgomery_xzdouble; curve25519x; PAIR_EQ] THEN
-    REWRITE_TAC[GSYM RING_OF_INT_OF_NUM; RING_OF_INT_CLAUSES] THEN
-    ASM_REWRITE_TAC[RING_OF_INT_EQ] THEN
-    REWRITE_TAC[GSYM INT_OF_NUM_REM; GSYM INT_REM_EQ;
-                GSYM INT_OF_NUM_CLAUSES] THEN
-    ASM_REWRITE_TAC[] THEN CONV_TAC INT_REM_DOWN_CONV THEN
-    REPEAT CONJ_TAC THEN AP_THM_TAC THEN AP_TERM_TAC THEN
-    REWRITE_TAC[A_25519] THEN INT_ARITH_TAC;
-    FIRST_X_ASSUM(K ALL_TAC o check (is_forall o concl)) THEN
+    ASM_REWRITE_TAC[GSYM INT_REM_EQ] THEN CONV_TAC INT_REM_DOWN_CONV THEN
+    ASM_REWRITE_TAC[montgomery_xzdouble; montgomery_xzdiffadd;
+                    curve25519; A_25519; INTEGER_MOD_RING_CLAUSES] THEN
+    CONV_TAC INT_REM_DOWN_CONV THEN
+    REPEAT CONJ_TAC THEN AP_THM_TAC THEN AP_TERM_TAC THEN INT_ARITH_TAC;
     REPEAT(FIRST_X_ASSUM(K ALL_TAC o check
      (fun th -> intersect (frees (concl th))
-                [`xn2:num`; `zn2:num`; `d:num`; `d':num`;
+                [`xn2:num`; `zn2:num`;  `d:num`; `d':num`;
                  `s:num`; `s':num`; `p:num`; `e:num`] <> []))) THEN
     STRIP_TAC] THEN
-
-  (*** Clean up final goal and observe that we've reached nn ***)
-
-  SUBGOAL_THEN `2 * 2 * 2 * nn DIV 8 = nn` SUBST_ALL_TAC THENL
-   [REWRITE_TAC[ARITH_RULE `2 * 2 * 2 * nn DIV 8 = nn <=> nn MOD 8 = 0`] THEN
-    EXPAND_TAC "nn" THEN
-    REWRITE_TAC[ARITH_RULE `2 EXP 254 = 8 * 2 EXP 251`; MOD_MULT_MOD] THEN
-    REWRITE_TAC[ADD_SUB; GSYM LEFT_ADD_DISTRIB; MOD_MULT];
-    ALL_TAC] THEN
-
-  SUBGOAL_THEN `X < 2 * p_25519` ASSUME_TAC THENL
-   [FIRST_X_ASSUM(MP_TAC o MATCH_MP (ARITH_RULE
-     `Y MOD 2 EXP 255 = X ==> X < 2 EXP 255`)) THEN
-    REWRITE_TAC[p_25519] THEN ARITH_TAC;
-    ALL_TAC] THEN
-
-  REPEAT(FIRST_X_ASSUM(K ALL_TAC o
-   check (vfree_in `n_input:num`) o concl)) THEN
-  REPEAT(FIRST_X_ASSUM(K ALL_TAC o
-   check (vfree_in `X_input:num`) o concl)) THEN
 
   (*** The inlining of modular inverse ***)
 
   ARM_STEPS_TAC CURVE25519_X25519_BYTE_ALT_EXEC (36--37) THEN
   LOCAL_MODINV_TAC 38 THEN
-  FIRST_X_ASSUM(ASSUME_TAC o MATCH_MP(MESON[PRIME_COPRIME_EQ; PRIME_P25519]
-   `(bnx = if p_25519 divides n then 0 else inverse_mod p_25519 n)
-    ==> coprime(p_25519,n) ==> bnx = inverse_mod p_25519 n`)) THEN
-  ABBREV_TAC
-   `zn' =
-    read(memory :> bytes(word_add stackpointer (word 224),8 * 4)) s38` THEN
 
-  (*** The tweaking to force xn = 0 whenever zn = 0 ***)
+  (*** The final multiplication ***)
 
-  BIGNUM_LDIGITIZE_TAC "xn_"
-   `read(memory :> bytes(word_add stackpointer (word 288),8 * 4)) s38` THEN
-  BIGNUM_LDIGITIZE_TAC "zn_"
-   `read(memory :> bytes(word_add stackpointer (word 160),8 * 4)) s38` THEN
-  ARM_STEPS_TAC CURVE25519_X25519_BYTE_ALT_EXEC (39--52) THEN
-
-  SUBGOAL_THEN
-   `read(memory :> bytes(word_add stackpointer (word 288),8 * 4)) s52 =
-    if zn = 0 then 0 else xn`
-  ASSUME_TAC THENL
-   [CONV_TAC(ONCE_DEPTH_CONV BIGNUM_LEXPAND_CONV) THEN
-    ASM_REWRITE_TAC[] THEN MAP_EVERY EXPAND_TAC ["zn"; "xn"] THEN
-    REWRITE_TAC[WORD_SUB_0; VAL_EQ_0; WORD_OR_EQ_0] THEN
-    REWRITE_TAC[BIGNUM_OF_WORDLIST_EQ_0; ALL] THEN
-    REWRITE_TAC[COND_SWAP; CONJ_ACI] THEN
-    COND_CASES_TAC THEN ASM_REWRITE_TAC[] THEN
-    REWRITE_TAC[bignum_of_wordlist] THEN
-    CONV_TAC(DEPTH_CONV WORD_NUM_RED_CONV);
-    ALL_TAC] THEN
-
-  (*** Final multiplication ***)
-
-  LOCAL_MUL_P25519_TAC 0 ["zn"; "xn"; "xm"] THEN
+  LOCAL_MUL_P25519_TAC 0 ["zn"; "xn"; "zn"] THEN
 
   (*** Bytewise store and finish of simulation ***)
 
   BIGNUM_LDIGITIZE_TAC "res_"
-   `read(memory :> bytes(word_add stackpointer (word 160),8 * 4)) s53` THEN
-  ARM_STEPS_TAC CURVE25519_X25519_BYTE_ALT_EXEC (54--115) THEN
+   `read(memory :> bytes(word_add stackpointer (word 160),8 * 4)) s39` THEN
+  ARM_STEPS_TAC CURVE25519_X25519_BYTE_ALT_EXEC (40--101) THEN
   ENSURES_FINAL_STATE_TAC THEN ASM_REWRITE_TAC[] THEN
-  TRANS_TAC EQ_TRANS `zn'':num` THEN CONJ_TAC THENL
-   [CONV_TAC(LAND_CONV BYTES_EXPAND_CONV) THEN EXPAND_TAC "zn''" THEN
+  TRANS_TAC EQ_TRANS `zn':num` THEN CONJ_TAC THENL
+   [CONV_TAC(LAND_CONV BYTES_EXPAND_CONV) THEN EXPAND_TAC "zn'" THEN
     REWRITE_TAC[bignum_of_wordlist] THEN ASM_REWRITE_TAC[] THEN
     REWRITE_TAC[bignum_of_wordlist; val_def] THEN
     REWRITE_TAC[DIMINDEX_8; ARITH_RULE `i < 8 <=> 0 <= i /\ i <= 7`] THEN
@@ -5661,84 +5559,15 @@ let CURVE25519_X25519_BYTE_ALT_CORRECT = time prove
     CONV_TAC(DEPTH_CONV WORD_NUM_RED_CONV) THEN ARITH_TAC;
     ASM_REWRITE_TAC[]] THEN
 
-  (*** Completing the mathematics ***)
+  (*** Finishing the mathematics ***)
 
-  CONV_TAC SYM_CONV THEN MATCH_MP_TAC PUREX25519_UNIQUE_IMP THEN
-  CONJ_TAC THENL [REWRITE_TAC[MOD_LT_EQ; p_25519] THEN ARITH_TAC; ALL_TAC] THEN
-  MAP_EVERY X_GEN_TAC [`f:(int#int)ring`; `P:((int#int)#(int#int))option`] THEN
-
-  ASM_CASES_TAC `X MOD p_25519 = 0` THEN
-  ASM_REWRITE_TAC[RING_OF_NUM_0] THEN STRIP_TAC THENL
-   [MP_TAC(ISPECL
-     [`f:(int#int)ring`; `ring_of_num f A_25519:int#int`;
-      `ring_of_num f 1:int#int`; `P:((int#int)#(int#int))option`;
-      `nn:num`] MONTGOMERY_XMAP_EQ_0_POW) THEN
-    ASM_REWRITE_TAC[GSYM curve25519x_group; GSYM curve25519x] THEN
-    ASM_SIMP_TAC[MONTGOMERY_NONSINGULAR_CURVE25519X; RING_OF_NUM] THEN
-    ANTS_TAC THENL [REWRITE_TAC[p_25519] THEN ARITH_TAC; ALL_TAC] THEN
-    DISCH_THEN SUBST1_TAC THEN FIRST_X_ASSUM(MP_TAC o SPECL
-     [`f:(int#int)ring`; `SOME(ring_0 f:int#int,ring_0 f)`]) THEN
-    ASM_REWRITE_TAC[] THEN ANTS_TAC THENL
-     [REWRITE_TAC[curve25519x_halfcanonically_represents] THEN
-      ASM_SIMP_TAC[CURVE25519X_GROUP; montgomery_xz] THEN
-      GEN_REWRITE_TAC LAND_CONV [IN] THEN
-      REWRITE_TAC[montgomery_curve; RING_OF_NUM; curve25519x] THEN
-      ONCE_REWRITE_TAC[GSYM RING_OF_NUM_MOD] THEN ASM_REWRITE_TAC[] THEN
-      REWRITE_TAC[p_25519; A_25519] THEN CONV_TAC NUM_REDUCE_CONV THEN
-      ASM_SIMP_TAC[RING_OF_NUM_1; RING_OF_NUM_0; FIELD_NONTRIVIAL; RING_0] THEN
-      UNDISCH_TAC `field(f:(int#int)ring)` THEN POP_ASSUM_LIST(K ALL_TAC) THEN
-      REPEAT STRIP_TAC THEN FIELD_TAC;
-      ASM_SIMP_TAC[MOD_LT]] THEN
-    COND_CASES_TAC THEN
-    ASM_REWRITE_TAC[MOD_0; RING_OF_NUM_0; MULT_CLAUSES] THEN
-    ONCE_REWRITE_TAC[GSYM MOD_MULT_MOD2] THEN
-    SIMP_TAC[MOD_0; RING_OF_NUM_0; MULT_CLAUSES];
-    ALL_TAC] THEN
-
-  FIRST_X_ASSUM(MP_TAC o SPECL
-   [`f:(int#int)ring`; `P:((int#int)#(int#int))option`]) THEN
-  ASM_REWRITE_TAC[] THEN ANTS_TAC THENL
-   [ASM_REWRITE_TAC[curve25519x_halfcanonically_represents] THEN
-    REWRITE_TAC[p_25519] THEN CONV_TAC NUM_REDUCE_CONV THEN
-    REWRITE_TAC[RING_OF_NUM_1] THEN
-    W(MP_TAC o PART_MATCH (lhand o rand) MONTGOMERY_XZ_XMAP o snd) THEN
-    ASM_REWRITE_TAC[RING_OF_NUM] THEN
-    ONCE_REWRITE_TAC[GSYM RING_OF_NUM_MOD] THEN
-    ASM_REWRITE_TAC[MOD_MOD_REFL] THEN
-    DISCH_THEN MATCH_MP_TAC THEN
-    ASM_REWRITE_TAC[RING_OF_NUM_EQ_0; DIVIDES_MOD] THEN
-    ASM_SIMP_TAC[MOD_LT; MOD_MOD_REFL];
-    ALL_TAC] THEN
-
-  REWRITE_TAC[curve25519x_halfcanonically_represents] THEN
-  REPEAT(DISCH_THEN(CONJUNCTS_THEN2 ASSUME_TAC MP_TAC)) THEN
-  FIRST_X_ASSUM(MP_TAC o SPEC `nn:num` o MATCH_MP GROUP_POW) THEN
-  SPEC_TAC(`group_pow (curve25519x_group(f:(int#int)ring)) P nn`,
-           `Q:((int#int)#(int#int))option`) THEN
-  REWRITE_TAC[FORALL_OPTION_THM] THEN
-  GEN_REWRITE_TAC RAND_CONV [FORALL_PAIR_THM] THEN
-  REWRITE_TAC[montgomery_xz; montgomery_xmap] THEN
-  ASM_SIMP_TAC[RING_OF_NUM_EQ_0; DIVIDES_MOD; MOD_LT] THEN
-  REWRITE_TAC[RING_OF_NUM] THEN ONCE_REWRITE_TAC[IN] THEN
-  ASM_SIMP_TAC[CURVE25519X_GROUP] THEN
-  REWRITE_TAC[montgomery_curve; curve25519x] THEN
-  SIMP_TAC[MULT_CLAUSES; MOD_0; RING_OF_NUM_0] THEN
-  MAP_EVERY X_GEN_TAC [`u:int#int`; `v:int#int`] THEN
-  STRIP_TAC THEN
-  DISCH_THEN(CONJUNCTS_THEN2 ASSUME_TAC (SUBST1_TAC o SYM)) THEN
-  MP_TAC(ISPEC `f:(int#int)ring` RING_OF_NUM_MOD) THEN
-  ASM_SIMP_TAC[RING_OF_NUM_MUL] THEN DISCH_THEN(K ALL_TAC) THEN
-  REWRITE_TAC[ring_div] THEN AP_TERM_TAC THEN
-  MATCH_MP_TAC RING_RINV_UNIQUE THEN
-  REWRITE_TAC[RING_OF_NUM; GSYM RING_OF_NUM_MUL] THEN
-  REWRITE_TAC[GSYM RING_OF_NUM_1; RING_OF_NUM_EQ] THEN
-  FIRST_X_ASSUM(MP_TAC o check (is_imp o concl)) THEN
-  ASM_REWRITE_TAC[] THEN
-  MATCH_MP_TAC(TAUT `(p /\ q ==> r) /\ p ==> (p ==> q) ==> r`) THEN
-  CONJ_TAC THENL [MESON_TAC[INVERSE_MOD_RMUL]; ALL_TAC] THEN
-  SIMP_TAC[PRIME_COPRIME_EQ; PRIME_P25519] THEN
-  ASM_SIMP_TAC[DIVIDES_MOD; MOD_LT] THEN
-  REWRITE_TAC[p_25519] THEN CONV_TAC NUM_REDUCE_CONV);;
+  CONV_TAC SYM_CONV THEN REWRITE_TAC[GSYM deproject; PUREX25519_MOD] THEN
+  MATCH_MP_TAC DEPROJECT_LADDER_EVEN THEN ASM_REWRITE_TAC[] THEN
+  REPEAT(CONJ_TAC THENL [EXPAND_TAC "nn" THEN ARITH_TAC; ALL_TAC]) THEN
+  REWRITE_TAC[GSYM DIVIDES_2] THEN
+  FIRST_X_ASSUM(MATCH_MP_TAC o MATCH_MP (REWRITE_RULE[IMP_CONJ_ALT]
+        DIVIDES_TRANS)) THEN
+  REWRITE_TAC[DIVIDES_MOD] THEN ARITH_TAC);;
 
 let CURVE25519_X25519_BYTE_ALT_SUBROUTINE_CORRECT = time prove
  (`!res scalar n point X pc stackpointer returnaddress.
